semantics/replScript.sml
@@ -130,8 +130,8 @@ val (ast_repl_rules, ast_repl_ind, ast_repl_cases) = Hol_reln `
 (!state type_errors ast asts top rest type_bindings' ctors' tenvM' tenvC' tenv' store' r.
   (elab_top state.type_bindings state.ctors ast = 
    (type_bindings', ctors', top)) ∧
-  (type_prog state.tenvM state.tenvC state.tenv [top] tenvM' tenvC' tenv') ∧
-  evaluate_prog state.envM state.envC state.store state.envE [top] (store',r) ∧
+  (type_top state.tenvM state.tenvC state.tenv top tenvM' tenvC' tenv') ∧
+  evaluate_top state.envM state.envC state.store state.envE top (store',r) ∧
   ast_repl (update_repl_state state type_bindings' ctors' tenvM' tenvC' tenv' store' r) type_errors asts rest
   ⇒
   ast_repl state (F::type_errors) (SOME ast::asts) (Result (print_result r) rest)) ∧
@@ -139,8 +139,8 @@ val (ast_repl_rules, ast_repl_ind, ast_repl_cases) = Hol_reln `
 (!state type_errors ast asts top type_bindings' ctors' tenvM' tenvC' tenv'.
   (elab_top state.type_bindings state.ctors ast = 
    (type_bindings', ctors', top)) ∧
-  (type_prog state.tenvM state.tenvC state.tenv [top] tenvM' tenvC' tenv') ∧
-  prog_diverges state.envM state.envC state.store state.envE [top]
+  (type_top state.tenvM state.tenvC state.tenv top tenvM' tenvC' tenv') ∧
+  top_diverges state.envM state.envC state.store state.envE top
   ⇒
   ast_repl state (F::type_errors) (SOME ast::asts) Diverge) ∧
 
